Refactored combination proofs.

progs/io_combine.v
@@ -20,306 +20,12 @@ Notation "t1 ;; t2" := (ITree.bind t1 (fun _ => t2))
 Notation "' p <- t1 ;; t2" :=
   (ITree.bind t1 (fun x_ => match x_ with p => t2 end))
 (at level 100, t1 at next level, p pattern, right associativity) : itree_scope.
-
-(*Section ext_safe.
-
-  Context {Espec : OracleKind} {OS_state : Type} {etrace : Type}.
-  Variable prog : Clight.program.
-  Variable ext_sem : external_function -> list val -> OS_state -> OS_state * option val * etrace.
-  Variable consume_trace : OK_ty -> OK_ty -> etrace -> Prop.
-  Variable inj_mem : mem -> OS_state -> Prop.
-  Variable extr_mem : OS_state -> mem.
-  Notation ge := (globalenv prog).
-
-  Inductive ext_safeN : nat -> OK_ty -> corestate -> mem -> Prop :=
-  | ext_safeN_0: forall z c m, ext_safeN O z c m
-  | ext_safeN_step:
-      forall n z c m c' m',
-      cl_step ge c m c' m' ->
-      ext_safeN n z c' m' ->
-      ext_safeN (S n) z c m
-  | ext_safeN_external:
-      forall n z c m e args,
-      cl_at_external c = Some (e,args) ->
-      (forall s s' ret m' t' n'
-         (Hargsty : Val.has_type_list args (sig_args (ef_sig e)))
-         (Hretty : step_lemmas.has_opttyp ret (sig_res (ef_sig e))),
-         inj_mem m s ->
-         ext_sem e args s = (s', ret, t') ->
-         m' = extr_mem s' ->
-         (n' <= n)%nat ->
-         exists z' c', consume_trace z z' t' /\
-           cl_after_external ret c = Some c' /\
-           ext_safeN n' z' c' m') ->
-      ext_safeN (S n) z c m.
-
-  Variable dryspec : ext_spec OK_ty.
-  Hypothesis extcalls_correct : forall e w b tl args z m s, ext_spec_pre dryspec e w b tl args z m ->
-    inj_mem m s ->
-    let '(s', ret, t') := ext_sem e args s in
-    exists z', consume_trace z z' t' /\
-    ext_spec_post dryspec e w b (sig_res (ef_sig e)) ret z' (extr_mem s').
-
-  Lemma dry_safe_ext_safe : forall n z q m,
-    step_lemmas.dry_safeN(genv_symb := Clight_sim.genv_symb_injective)
-     (Clight_sim.coresem_extract_cenv (cl_core_sem (globalenv prog)) (prog_comp_env prog)) dryspec
-     (Build_genv (Genv.globalenv prog) (prog_comp_env prog)) n z q m ->
-    ext_safeN n z q m.
-  Proof.
-    induction n as [n IHn] using lt_wf_ind; intros; inversion H; subst; try contradiction.
-    - constructor.
-    - econstructor; eauto.
-    - eapply ext_safeN_external; eauto; intros.
-      eapply extcalls_correct in H1; eauto.
-      rewrite H4 in H1; destruct H1 as (z' & ? & ?).
-      edestruct H2 as (? & ? & ?); eauto.
-      do 3 eexists; eauto; split; eauto.
-      subst; apply IHn; auto; omega.
-  Qed.
-
-  Theorem OS_safety:
-   forall {CS: compspecs} (initial_oracle: OK_ty)
-     (dessicate : forall (ef : external_function) jm,
-               ext_spec_type OK_spec ef ->
-               ext_spec_type dryspec ef)
-     (JDE: juicy_dry_ext_spec _ (@JE_spec OK_ty OK_spec) dryspec dessicate)
-     (DME: ext_spec_mem_evolve _ dryspec)
-     V G m,
-     @semax_prog_ext Espec CS prog initial_oracle V G ->
-     Genv.init_mem prog = Some m ->
-     exists b, exists q, exists m',
-       Genv.find_symbol (Genv.globalenv prog) (prog_main prog) = Some b /\
-       initial_core  (cl_core_sem (globalenv prog))
-           0 m q m' (Vptr b Ptrofs.zero) nil /\
-       forall n, ext_safeN n initial_oracle q m'.
-  Proof.
-    intros.
-    eapply CSHL_Sound.semax_prog_ext_sound, whole_program_sequential_safety_ext in H as (b & q & m' & ? & ? & Hsafe); eauto.
-    do 4 eexists; eauto; split; eauto; intro n.
-    eapply dry_safe_ext_safe; eauto.
-  Qed.
-
-End ext_safe.*)
-
 Require Import ITree.Interp.Traces.
 Require Import Ensembles.
-
-Section ext_trace.
-
-  Context {cevent : Type -> Type} {J : juicy_ext_spec (itree cevent unit)} {OS_state : Type} {event : Type}.
-  Variable prog : Clight.program.
-  Variable ext_sem : external_function -> list val -> OS_state -> option (OS_state * option val * list event).
-  Variable inj_mem : mem -> OS_state -> Prop.
-  Variable extr_mem : OS_state -> mem.
-  Notation ge := (globalenv prog).
-
-  Instance Espec : OracleKind := Build_OracleKind (itree cevent unit) J.
-
-  Variable lift_event : event -> {X & option (cevent X * X)%type}.
-
-  Fixpoint trace_of_events (t : list event) : @trace cevent unit :=
-    match t with
-    | nil => TEnd
-    | e :: t' =>
-        match projT2 (lift_event e) with
-        | Some (e', r) => TEventResponse e' r (trace_of_events t')
-        | None => trace_of_events t'
-        end
-    end.
-
-  Definition consume_trace (z z' : itree cevent unit) le := let t := trace_of_events le in
-    forall t', is_trace z' t' -> is_trace z (app_trace t t').
-
-(*  Inductive ext_traceN : nat -> list event -> OK_ty -> corestate -> mem -> Prop :=
-  | ext_traceN_0: forall z c m, ext_traceN O [] z c m
-  | ext_traceN_step:
-      forall n t z c m c' m',
-      cl_step ge c m c' m' ->
-      ext_traceN n t z c' m' ->
-      ext_traceN (S n) t z c m
-  | ext_traceN_external:
-      forall n z c m e args,
-      cl_at_external c = Some (e,args) ->
-      forall s s' ret m' t t' n'
-       (Hargsty : Val.has_type_list args (sig_args (ef_sig e)))
-       (Hretty : step_lemmas.has_opttyp ret (sig_res (ef_sig e))),
-       inj_mem m s ->
-       ext_sem e args s = (s', ret, t) ->
-       m' = extr_mem s' ->
-       (n' <= n)%nat ->
-       forall z' c', consume_trace z z' t ->
-       cl_after_external ret c = Some c' ->
-       ext_traceN n' t' z' c' m' ->
-      ext_traceN (S n) (t ++ t') z c m.*)
-
-  Lemma consume_trace_nil : forall z, consume_trace z z nil.
-  Proof.
-    repeat intro; auto.
-  Qed.
-
-  Lemma trace_of_events_app : forall t t', trace_of_events (t ++ t') = app_trace (trace_of_events t) (trace_of_events t').
-  Proof.
-    induction t; auto; simpl; intros.
-    destruct (lift_event a) as (? & [(? & ?) |]); simpl; auto.
-    rewrite IHt; auto.
-  Qed.
-
-  Lemma app_trace_assoc : forall {E : Type -> Type} {R : Type} (t t' t'' : @trace E R),
-    app_trace (app_trace t t') t'' = app_trace t (app_trace t' t'').
-  Proof.
-    induction t; auto; simpl; intros.
-    rewrite IHt; auto.
-  Qed.
-
-  Lemma consume_trace_app : forall z z' z'' t t', consume_trace z z' t -> consume_trace z' z'' t' ->
-    consume_trace z z'' (t ++ t').
-  Proof.
-    unfold consume_trace; intros.
-    rewrite trace_of_events_app, app_trace_assoc; auto.
-  Qed.
-
-(*  Theorem ext_trace_correct:
-   forall (initial_oracle: OK_ty) q m n t,
-    ext_traceN n t initial_oracle q m ->
-    exists z', consume_trace initial_oracle z' t.
-  Proof.
-    induction 1.
-    - exists z; repeat intro; auto.
-    - auto.
-    - destruct IHext_traceN as [z'' ?].
-      exists z''.
-      eapply consume_trace_app; eauto.
-  Qed.*)
-
-  Inductive ext_safeN_trace : nat -> Ensemble (list event) -> OK_ty -> corestate -> mem -> Prop :=
-  | ext_safeN_trace_0: forall z c m, ext_safeN_trace O (Empty_set _) z c m
-  | ext_safeN_trace_step:
-      forall n traces z c m c' m',
-      cl_step ge c m c' m' ->
-      ext_safeN_trace n traces z c' m' ->
-      ext_safeN_trace (S n) traces z c m
-  | ext_safeN_trace_external:
-      forall n traces z c m e args,
-      cl_at_external c = Some (e,args) ->
-      (forall s s' ret m' t n'
-         (Hargsty : Val.has_type_list args (sig_args (ef_sig e)))
-         (Hretty : step_lemmas.has_opttyp ret (sig_res (ef_sig e))),
-         inj_mem m s ->
-         ext_sem e args s = Some (s', ret, t) ->
-         m' = extr_mem s' ->
-         (n' <= n)%nat ->
-         exists traces' z' c', consume_trace z z' t /\
-           cl_after_external ret c = Some c' /\
-           ext_safeN_trace n' traces' z' c' m' /\
-           (forall t', In _ traces' t' -> In _ traces (t ++ t'))) ->
-      (forall t1, In _ traces t1 ->
-        exists s s' ret m' t n', Val.has_type_list args (sig_args (ef_sig e)) /\
-         step_lemmas.has_opttyp ret (sig_res (ef_sig e)) /\
-         inj_mem m s /\ ext_sem e args s = Some (s', ret, t) /\ m' = extr_mem s' /\
-         (n' <= n)%nat /\ exists traces' z' c', consume_trace z z' t /\
-           cl_after_external ret c = Some c' /\ ext_safeN_trace n' traces' z' c' m' /\
-        exists t', In _ traces' t' /\ t1 = t ++ t') ->
-      ext_safeN_trace (S n) traces z c m.
-
-  Variable dryspec : ext_spec OK_ty.
-  Hypothesis extcalls_correct : forall e w b tl args z m s, ext_spec_pre dryspec e w b tl args z m ->
-    inj_mem m s ->
-    forall s' ret t', Some (s', ret, t') = ext_sem e args s ->
-    exists z', consume_trace z z' t' /\
-    ext_spec_post dryspec e w b (sig_res (ef_sig e)) ret z' (extr_mem s').
-
-  Lemma dry_safe_ext_trace_safe : forall n z q m,
-    step_lemmas.dry_safeN(genv_symb := Clight_sim.genv_symb_injective)
-     (Clight_sim.coresem_extract_cenv (cl_core_sem (globalenv prog)) (prog_comp_env prog)) dryspec
-     (Build_genv (Genv.globalenv prog) (prog_comp_env prog)) n z q m ->
-    exists traces, ext_safeN_trace n traces z q m.
-  Proof.
-    induction n as [n IHn] using lt_wf_ind; intros; inversion H; subst; try contradiction.
-    - eexists; constructor.
-    - edestruct IHn as [traces ?]; eauto; exists traces; econstructor; eauto.
-    - exists (fun t1 => exists s s' ret m' t n', Val.has_type_list args (sig_args (ef_sig e)) /\
-         step_lemmas.has_opttyp ret (sig_res (ef_sig e)) /\
-         inj_mem m s /\ ext_sem e args s = Some (s', ret, t) /\ m' = extr_mem s' /\
-         (n' <= n0)%nat /\ exists traces' z' c', consume_trace z z' t /\
-           cl_after_external ret q = Some c' /\ ext_safeN_trace n' traces' z' c' m' /\
-        exists t', In _ traces' t' /\ t1 = t ++ t').
-      eapply ext_safeN_trace_external; eauto; intros.
-      eapply extcalls_correct in H1; eauto.
-      destruct H1 as (z' & ? & ?).
-      edestruct H2 as (? & ? & Hsafe); eauto.
-      apply IHn in Hsafe as [traces ?]; [|omega].
-      subst; do 4 eexists; eauto; split; eauto; split; eauto.
-      intros; unfold In.
-      do 7 eexists; eauto; split; eauto; split; eauto; split; eauto; split; eauto; split; eauto.
-      do 4 eexists; eauto.
-  Qed.
-
-  Lemma safety_trace:
-   forall {CS: compspecs} (initial_oracle: OK_ty)
-     (dessicate : forall (ef : external_function) jm,
-               ext_spec_type OK_spec ef ->
-               ext_spec_type dryspec ef)
-     (JDE: juicy_dry_ext_spec _ (@JE_spec OK_ty OK_spec) dryspec dessicate)
-     (DME: ext_spec_mem_evolve _ dryspec)
-     V G m,
-     @semax_prog_ext Espec CS prog initial_oracle V G ->
-     Genv.init_mem prog = Some m ->
-     exists b, exists q, exists m',
-       Genv.find_symbol (Genv.globalenv prog) (prog_main prog) = Some b /\
-       initial_core  (cl_core_sem (globalenv prog))
-           0 m q m' (Vptr b Ptrofs.zero) nil /\
-       forall n, exists traces, ext_safeN_trace n traces initial_oracle q m'.
-  Proof.
-    intros.
-    eapply CSHL_Sound.semax_prog_ext_sound, whole_program_sequential_safety_ext in H as (b & q & m' & ? & ? & Hsafe); eauto.
-    do 4 eexists; eauto; split; eauto; intro n.
-    eapply dry_safe_ext_trace_safe; eauto.
-  Qed.
-
-  Lemma trace_correct:
-   forall n (z: OK_ty) q m traces t,
-    ext_safeN_trace n traces z q m ->
-    In _ traces t ->
-    exists z', consume_trace z z' t.
-  Proof.
-    induction n as [n IHn] using lt_wf_ind; intros; inversion H; subst.
-    - inversion H0.
-    - eauto.
-    - destruct (H3 _ H0) as (s & s' & ret & m' & t1 & n' & ? & ? & ? & ? & ? & ? & traces' & z' & c' & ? & ? & ? & ? & ? & ?).
-      edestruct (IHn n') as [z'' ?]; eauto; [omega|].
-      subst; eexists; eapply consume_trace_app; eauto.
-  Qed.
-
-  Theorem OS_soundness:
-   forall {CS: compspecs} (initial_oracle: OK_ty)
-     (dessicate : forall (ef : external_function) jm,
-               ext_spec_type OK_spec ef ->
-               ext_spec_type dryspec ef)
-     (JDE: juicy_dry_ext_spec _ (@JE_spec OK_ty OK_spec) dryspec dessicate)
-     (DME: ext_spec_mem_evolve _ dryspec)
-     V G m,
-     @semax_prog_ext Espec CS prog initial_oracle V G ->
-     Genv.init_mem prog = Some m ->
-     exists b, exists q, exists m',
-       Genv.find_symbol (Genv.globalenv prog) (prog_main prog) = Some b /\
-       initial_core  (cl_core_sem (globalenv prog))
-           0 m q m' (Vptr b Ptrofs.zero) nil /\
-       forall n, exists traces, ext_safeN_trace n traces initial_oracle q m' /\
-         forall t, In _ traces t -> exists z', consume_trace initial_oracle z' t.
-  Proof.
-    intros.
-    eapply safety_trace in H as (b & q & m' & ? & ? & Hsafe); eauto.
-    exists b, q, m'; split; auto; split; auto.
-    intro n; destruct (Hsafe n) as [traces Hsafen].
-    exists traces; split; auto.
-    intros; eapply trace_correct; eauto.
-  Qed.
-
-End ext_trace.
-
 Require Import VST.progs.io_dry.
 Require Import VST.progs.io_os_connection.
 Require Import VST.progs.io_os_specs.
+Require Import VST.progs.os_combine.
 
 Section IO_safety.
 
@@ -328,23 +34,32 @@ Variable (prog : Clight.program).
 
 Definition ext_link := ext_link_prog prog.
 
-Definition sys_getc_wrap_spec (abd : RData) : option (RData * val * ostrace) :=
+Definition sys_getc_wrap_spec (abd : RData) : option (RData * val * trace) :=
   match sys_getc_spec abd with
-  | Some abd' => Some (abd', get_sys_ret abd', strip_common_prefix IOEvent_eq abd.(io_log) abd'.(io_log))
+  | Some abd' => Some (abd', get_sys_ret abd', trace_of_ostrace (strip_common_prefix IOEvent_eq abd.(io_log) abd'.(io_log)))
+  | None => None
+  end.
+
+Definition sys_putc_wrap_spec (abd : RData) : option (RData * val * trace) :=
+  match sys_putc_spec abd with
+  | Some abd' => Some (abd', get_sys_ret abd', trace_of_ostrace (strip_common_prefix IOEvent_eq abd.(io_log) abd'.(io_log)))
   | None => None
   end.
 
 Definition IO_ext_sem e (args : list val) s :=
   if oi_eq_dec (Some (ext_link "putchar"%string, funsig2signature ([(1%positive, tint)], tint) cc_default))
     (ef_id_sig ext_link e) then
-    (* putchar_spec (Znth 0 args) s *) Some (s, None, []) else
+    match sys_putc_wrap_spec s with
+    | Some (s', ret, t') => Some (s', Some ret, t')
+    | None => None
+    end else
   if oi_eq_dec  (Some (ext_link "getchar"%string, funsig2signature ([], tint) cc_default))
     (ef_id_sig ext_link e) then
     match sys_getc_wrap_spec s with
     | Some (s', ret, t') => Some (s', Some ret, t')
     | None => None
     end
-  else Some (s, None, []).
+  else Some (s, None, TEnd).
 
 Definition IO_inj_mem (m : mem) s := valid_trace s. (* stub *)
 Definition OS_mem (s : RData) : mem := Mem.empty. (* stub *)
@@ -359,16 +74,20 @@ Theorem IO_OS_soundness:
    Genv.init_mem prog = Some m ->
    exists b, exists q, exists m',
      Genv.find_symbol (Genv.globalenv prog) (prog_main prog) = Some b /\
-     initial_core  (cl_core_sem (globalenv prog))
+     initial_core (cl_core_sem (globalenv prog))
          0 m q m' (Vptr b Ptrofs.zero) nil /\
-   forall n, exists traces, ext_safeN_trace(J := OK_spec) prog IO_ext_sem IO_inj_mem OS_mem lift_IO_event n traces initial_oracle q m' /\
-     forall t, In _ traces t -> exists z', consume_trace lift_IO_event initial_oracle z' t.
+   forall n, exists traces, ext_safeN_trace(J := OK_spec) prog IO_ext_sem IO_inj_mem OS_mem n traces initial_oracle q m' /\
+     forall t, In _ traces t -> exists z', consume_trace initial_oracle z' t.
 Proof.
   intros; eapply OS_soundness with (dryspec := io_dry_spec ext_link); eauto.
   - unfold IO_ext_sem; intros; simpl in *.
     if_tac; [|if_tac; [|contradiction]].
     + destruct w as (? & _ & ? & ?).
-      admit. (* need putchar_spec *)
+      destruct H2 as (? & ? & Hpre); subst.
+      destruct s; simpl in *.
+      unfold sys_putc_wrap_spec in *.
+      destruct (sys_putc_spec) eqn:Hspec; inv H4.
+      admit. (* need putc_correct *)
     + destruct w as (? & _ & ?).
       destruct H2 as (? & ? & Hpre); subst.
       destruct s; simpl in *.
